%%%%%%%%%%%%%%%%%%%%%%%%%%%%%%%%%%%%%%%%%
% Author: Sibi <sibi@psibi.in>
%%%%%%%%%%%%%%%%%%%%%%%%%%%%%%%%%%%%%%%%%
\documentclass{article}
\usepackage{graphicx}
\usepackage{verbatim}
\usepackage{amsmath}
\usepackage{amsfonts}
\usepackage{amssymb}
\usepackage{tabularx}
\setlength\parskip{\baselineskip}
\begin{document}
\title{Chapter 4 (Section 4.2)}
\author{Sibi}
\date{\today}
\maketitle
\newpage

\section{Problem 1}
Solution (a)

Domain = $\{ p \mid \text{p is a living parent} \}$
Range = $\{ q \mid \text{q is a living child} \}$

Solution(b)

Domain = $\mathbb{R}$
Range = $\mathbb{R^+}$

\section{Problem 2}

Solution(a)

Domain = $\{ p \mid \text{p is a brother to some living person }\}$
Range = $\{q \mid \text{q has some living brother.}\}$

Solution(b)

Domain = $\mathbb{R}$
Range = $\{ x \mid x \in \mathbb{R} \land  x > -1 \land x < 1 \}$

\section{Problem 3}

\subsection{Solution (a)}
\noindent

$L = \{(s,r) \in S \times R \mid \text{the student s lives in the dorm room
  r}\}$

$L^{-1} = \{(r,s} \in R \times S | (s,r) \in L\}$

$L^{-1} \circ L \text{ is relation on} S$

$L^{-1} \circ L = \{(s,t) \in S \times S \mid \exists r \in R((s,r) \in L \land
(r,t) \in L^{-1})\}$

$ = \{(s,t) \in S \times S \mid \exists r \in R (\text{ student s lives in
  dorm room r and so is student t})\}$

$ = \{(s,t) \in S \times S \mid \text{student s and t both live in some dorm
  room} \}$


\subsection{Solution b}
\noindent

$E \circ (L^{-1} \circ L)$ is relation from S to C.

$E \circ (L^{-1} \circ L) = \{(t,c) \in S \times C \mid \exists s \in
S((t,s) \in (S \times S) \land (s,c) \in S \times C\}$

\begin{multiline}
$=\{(t,c) \in S \times C \mid \exists s \in S(\text{ student s and t \\
  both live in some dorm room and student s is enrolled in course c})\}$
\end{multiline}

$=\{(t,c) \in S \times C \mid \text{ t is a student who shares the
    dorm \\ with another student who is enrolled in course c}\}$

\section{Problem 4}

\subsection{Solution (a)}
\noindent

$S \circ R = \{(a,b) \in A \times B \mid \exists c \in B((a,c) \in R
\land (c,b) \in S)$

$ = {(1,5), (1,6), (1,4), (2,4), (3,6)}$

\subsection{Solution (b)}
\noindent

$S \circ S^{- 1} = \{(a,b) \in B \times B \mid \exists c \in B((a,c)
\in S^{-1} \land (c,b) \in S\}$

$S \circ S^{- 1} = \{(a,b) \in B \times B \mid \exists c \in B((c,a)
\in S \land (c,b) \in S\}$

$ = \{(5,6),(6,5),(5,5),(6,6),(4,4)\}$

\section{Problem 5}

\subsection{Solution (a)}
\noindent
$S^{-1} \circ R = \{(a,b) \in A \times B \mid \exists c \in C((a,c)
\in R \land (c,b) \in S^{-1}\}$

$S^{-1} \circ R = \{(a,b) \in A \times B \mid \exists c \in C((a,c)
\in R \land (b,c) \in S\}$

= \{(1,4), (3,4), (3,5)\}

\subsection{Solution (b)}
\noindent
$R^{-1} \circ S = \{(b,a) \in B \times A \mid \exists c \in C((b,c)
\in S \land (c,a) \in R^{-1})\}$

$= \{(b,a) \in B \times A \exists c \in C((b,c) \in S \land (a,c) \in R\}$

$={(4,1),(4,3),(5,3)}$
\end{document}
