%%%%%%%%%%%%%%%%%%%%%%%%%%%%%%%%%%%%%%%%%
% Author: Sibi <sibi@psibi.in>
%%%%%%%%%%%%%%%%%%%%%%%%%%%%%%%%%%%%%%%%%
\documentclass{article}
\usepackage{graphicx}
\usepackage{verbatim}
\usepackage{amsmath}
\usepackage{amsfonts}
\usepackage{amssymb}
\usepackage{tabularx}
\setlength\parskip{\baselineskip}
\begin{document}
\title{Chapter 4 (Section 4.2)}
\author{Sibi}
\date{\today}
\maketitle
\newpage

\section{Problem 1}

$R = \{(a,bad), (a,cab), (b,bad), (b,bed), (b,cab), (c,cab), (d,bad),
(d, bed), (e,bed), (e,bed)\}$

\section{Problem 2}

$A = \{cat, dog, bird, rat\}$
$R = \{(x,y) \in A \times A \mid there is at least one letter that
occurs in both of the words x and y\}$

$R = \{(cat, cat), (cat, rat), (dog, dog), (dog, birds), (bird, dog),
(bird, bird), (bird, rat), (rat, cat), (rat, bird), (rat, rat)\}$

\begin{itemize}
\item Reflexive
\item Symmetric
\item Not transitive: there is an edge from bird to rat and rat to
  cat. But there is no edge from bird to cat.
\end{itemize}

\section{Problem 3}

$i_{A} = \{(x,y) \in A \times A \mid x = y\}$
$i_{A} = \{(1,1), (2,2), (3,3), (4,4)\}$

\section{Problem 4}

\subsection(Solution (a))

$R = \{(a,c), (c,c), (d,a), (d,b), (b,d)\}$

\begin{itemize}
\item Not reflexive since $(a,a) \notin R$
\item Not symmetric since $(a,c) \implies (c,a)$ doesn't hold
\item Not transitive since $(d,a) \land (d,c) \implies (d,c)$ doesn't hold
\end{itemize}

\subsection{Solution (b)}

$R = \{(a,b), (b,a), (a,d), (b,d)\}$

\begin{itemize}
\item Not reflexive since $(a,a) \notin R$
\item Not symmetric since $(a,d) \implies (d,a)$ doesn't hold
\item Not transitive since $(a,b) \land (b,a) \implies (a,a)$ doesn't hold
\end{itemize}

\subsection{Solution (c)}

$R = \{(a,a), (c,c), (b,b), (b,d), (d,b), (d,d)\}$

\begin{itemize}
\item Reflexive
\item Symmetric
\item Transitive
\end{itemize}

\subsection{Solution (d)}

$R = \{(a,c), (a,b), (a,d), (b,d), (c,d)\}$

\begin{itemize}
\item Not reflexive
\item Not symmetric
\item Transitive
\end{itemize}

\section{Solution 5}

$S \circ R = \{(a,c) \in A \times C \mid \exists b \in B((a,b) \in R
\land (b,c) \in S\}$

$S \circ R = \{(b,x), (a,y), (c,y), (a,z), (c,z)\}$

\section{Solution 6}

$ D_r = \{(x,y) \in R \times R \mid |x - y| < r \}$
$ D_s = \{(x,y) \in R \times R \mid |x - y| < s \}$

$ D_r \circ D_s = \{(a,b) \in R \times R \mid \exists c \in R((a,c)
\in D_s \land (c,b) \in D_r)\}$
$= \{(a,b) \in R \times R \mid \exists c \in R (|a - c| < s \land |c -
b| < r)\}$

From triangle inequality, $|a + b| < |a| + |b|$
$|(a-c) + (c-b)| < |a-c| + |c-b|$
$|a + (-b)| < s + r$
$ D_r \circ D_s = \{(a,b) \in R \times R \mid |a-b| < s + r\}$

\end{document}
